\begin{itemize}
    \item{
		\textbf{Propiedades de los Coeficientes Binomiales}
		\begin{itemize}
			\item{
				$C_k^n = C_{n-k}^n$
			}
			\item{
				$ C_0^n + C_1^n + C_2^n + \cdots + C_n^n = 2^n $
			}
			\item{
				$ C_0^n - C_1^n + C_2^n - \cdots + (-1)^n C_n^n = 0 $	
			}
			\item{
				$ \sum_{i=0}^n-1 = C_{k+1}^n $	
			}
			\item{
				$ C_n^n + C_n^n+1 + C_n^n+2 + \cdots + C_n^n+m-1 = C_{n+1}^{n+m} $
			}
		\end{itemize}
    }
    \item{
		\textbf{Propiedades de los Factoriales y las Permutaciones}
		\begin{itemize}
			\item{
				$ n! = (n-1)\bigl[(n-1)! + (n-2)!\bigr] $
			}
			\item{
				$ \sum_{n_1, n_2, \cdots n_k} P_(n_1, n_2, \cdots n_k) = k^n $
			}
		\end{itemize}
    }
    \item{
		\textbf{Subfactoriales}
		\begin{itemize}
			\item{
				$ D_n = P_n - C_1^n P_{n-1} + C_2^n P_{n-2} - \cdots + (-1)^n C_n^n $	
			}
			\item{
				$ D_n = n! \bigl[ 1 - \frac{1}{1!} + \frac{1}{2!} - \cdots + \frac{(-1)^n}{n!} \bigr]$	
			}
			\item{
				$ D_n = (n-1)[D_{n-1} + D_{n-2}] $ con $ D_0 = 1 $ y $ D_1 = 0 $	
			}
			\item{
				$D_n = n \cdot D_{n-1} + (-1)^n $
			}
		\end{itemize}
    }
\end{itemize}
